\documentclass[12pt]{article}
\usepackage{fullpage,graphicx,psfrag,url,ar,rotating,float}
\usepackage[small,bf]{caption}
\usepackage{amsmath,amssymb,enumitem,bbm,subcaption,multirow}
\setlength{\captionmargin}{20pt}
\setlist[enumerate]{label=(\roman*)}

\title{\Large{AA274 (Winter 2017-18): Problem Set 3}}
\author{Anqi Fu}

\begin{document}
\maketitle

\section{Extended Kalman Filter (EKF)}
\begin{enumerate}
	\item See submitted code. Let the state variables be $\mathbf{x}(t) = (x(t), y(t), \theta(t))$ and the control variables be $\mathbf{u}(t) = (V(t), \omega(t))$. The differential drive model is
	\begin{align*}
		\dot x(t) &= V(t)\cos(\theta(t)) \\
		\dot y(t) &= V(t)\sin(\theta(t)) \\
		\dot \theta(t) &= \omega(t),
	\end{align*}
	which we can discretize by assuming a zero-order hold on the control, i.e. $\mathbf{u}(t)$ is constant over a time interval of length $dt$. Then we can integrate to get
	\[
		\theta_t - \theta_{t-dt} = \int_{t-dt}^t \dot \theta(s)ds = \int_{t-dt}^t \omega(s)ds = \omega_t\int_{t-dt}^tds = \omega_tdt.
	\]
	If $\omega(t) = 0$ over the interval, $\theta(t)$ remains constant, so our coordinates can be found easily by integrating
	\begin{align*}
		x_t - x_{t-dt} &= \int_{t-dt}^t \dot x(s)ds = \int_{t-dt}^t V(s)\cos(\theta(s))ds = V_t\cos(\theta_{t-dt})dt \\
		y_t - y_{t-dt} &= \int_{t-dt}^t \dot y(s)ds = \int_{t-dt}^t V(s)\sin(\theta(s))ds = V_t\sin(\theta_{t-dt})dt.
	\end{align*}
	With a slight abuse of notation, We may thus write
	\[
		\mathbf{x}_t = \left(\begin{array}{c}
		x_t \\
		y_t \\
		\theta_t\end{array}\right) = \left(\begin{array}{c}
		x_{t-1} + V_t\cos(\theta_{t-1})dt \\
		y_{t-1} + V_t\sin(\theta_{t-1})dt \\
		\theta_{t-1} + \omega_tdt
		\end{array}\right) = g(\mathbf{x}_{t-1}, \mathbf{u}_t)
	\]
	and the Jacobians of $g$ with respect to $\mathbf{x}$ and $\mathbf{u}$ are, respectively,
	\[
		G_x = \left(\begin{array}{ccc}
		1 & 0 & -V_t\sin(\theta_{t-1})dt \\
		0 & 1 & V_t\cos(\theta_{t-1})dt \\
		0 & 0 & 1
		\end{array}\right) \quad \mbox{and} \quad
		G_u = \left(\begin{array}{cc}
		\cos(\theta_{t-1})dt & 0 \\
		\sin(\theta_{t-1})dt & 0 \\
		0 & dt
		\end{array}\right).
	\]
	If $\omega(t) \neq 0$, we exploit the fact that $\dot \theta(t) = \omega(t)$ to get
	\begin{align*}
		x_t - x_{t-dt} &= \int_{t-dt}^t V(s)\cos(\theta(s)) \frac{\dot \theta(s)}{\omega(s)}ds = \frac{V_t}{\omega_t}\int_{t-dt}^t \cos(\theta(s)) \dot \theta(s)ds \\
		&= \frac{V_t}{\omega_t} (\sin(\theta_t) - \sin(\theta_{t-dt})) = \frac{V_t}{\omega_t}(\sin(\theta_{t-dt}+ \omega_tdt) - \sin(\theta_{t-dt})) \\
		y_t - y_{t-dt} &= \frac{V_t}{\omega_t}\int_{t-dt}^t \sin(\theta(s))\dot \theta(s)ds = \frac{V_t}{\omega_t}(-\cos(\theta_{t-dt} + \omega_tdt) + \cos(\theta_{t-dt}))
	\end{align*}
	Our discrete model becomes
	\[
		\mathbf{x}_t = \left(\begin{array}{c}
		x_t \\
		y_t \\
		\theta_t\end{array}\right) = \left(\begin{array}{c}
		x_{t-1} + \frac{V_t}{\omega_t}(\sin(\theta_{t-1}+ \omega_tdt) - \sin(\theta_{t-1})) \\
		y_{t-1} - \frac{V_t}{\omega_t}(\cos(\theta_{t-1} + \omega_tdt) - \cos(\theta_{t-1})) \\
		\theta_{t-1} + \omega_tdt
		\end{array}\right) = g(\mathbf{x}_{t-1}, \mathbf{u}_t)
	\]
	with Jacobians
	\begin{align*}
		G_x &= \left(\begin{array}{ccc}
		1 & 0 & \frac{V_t}{\omega_t}(\cos(\theta_{t-1} + \omega_tdt) - \cos(\theta_{t-1})) \\
		0 & 1 & \frac{V_t}{\omega_t}(\sin(\theta_{t-1} + \omega_tdt) - \sin(\theta_{t-1})) \\
		0 & 0 & 1
		\end{array}\right) \\
		G_u &= \frac{1}{\omega_t}\left(\begin{array}{cc}
		\sin(\theta_t) - \sin(\theta_{t-1}) & -V_t(\frac{1}{\omega_t}(\sin(\theta_t) - \sin(\theta_{t-1})) - \cos(\theta_t)dt) \\
		-\cos(\theta_t) + \cos(\theta_{t-1}) & V_t(\frac{1}{\omega_t}(\cos(\theta_t) - \cos(\theta_{t-1})) + \sin(\theta_t)dt) \\
		0 & \omega_tdt
		\end{array}\right).
	\end{align*}
	where $\theta_t := \theta_{t-1} + \omega_tdt$.
	\item See submitted code. Let the belief state at $t-1$ be distributed as $\mathcal{N}(\mathbf{x}_{t-1}, P_{t-1})$. We model the dynamic certainty with white noise $\nu \sim \mathcal{N}(\mathbf{0}, Q)$ applied to the control input. For a time step of $dt$, the EKF prediction step is
	\begin{align*}
		\bar{\mathbf{x}}_t &= g(\mathbf{x}_{t-1}, \mathbf{u}_t) \\
		\bar P_t &= G_xP_{t-1}G_x^T + dt \cdot G_uQG_u^T.
	\end{align*}
	\item 
	\item 
	\item 
	\item 
	\item 
\end{enumerate}

\section{EKF Simultaneous Localization and Mapping (SLAM)}
\begin{enumerate}
	\item 
	\item 
	\item 
\end{enumerate}

\section{Turtlebot Localization}
\begin{enumerate}
	\item See submitted code.
	\item See submitted code.
\end{enumerate}

\end{document}